bootstrap/compile_repl_decsScript.sml
@@ -1,0 +1,47 @@
+open HolKernel boolLib bossLib cakeml_computeLib ml_repl_moduleTheory compile_primitivesTheory flookupLib
+val _ = new_theory"compile_repl_decs"
+
+val compile_repl_decs_def = zDefine`
+  compile_repl_decs = compile_top NONE (FST compile_primitives) (Tmod "REPL" NONE ml_repl_module_decls)`
+
+val _ = Globals.max_print_depth := 20
+
+val cs = cakeml_compset();
+(*TODO: add FUNION_FUPDATE_1 to finite_map compset*)
+val _ = computeLib.add_thms [finite_mapTheory.FUNION_FUPDATE_1,compile_primitives_eq] cs
+val _ = computeLib.scrub_const cs finite_mapSyntax.flookup_t;
+val _ = computeLib.add_conv (finite_mapSyntax.flookup_t,2,FLOOKUP_DEFN_CONV) cs;
+val eval = computeLib.CBV_CONV cs
+
+val compile_repl_decs_eq = save_thm("compile_repl_decs_eq",
+  time (REWR_CONV compile_repl_decs_def THENC PURE_ONCE_REWRITE_CONV[ml_repl_module_decls] THENC eval)
+  ``compile_repl_decs``)
+
+val repl_decs_code_def = zDefine
+  `repl_decs_code = code_labels real_inst_length (SND(SND(compile_repl_decs)))`
+
+val repl_decs_code_eq = save_thm("repl_decs_code_eq",
+  time (REWR_CONV repl_decs_code_def THENC PURE_ONCE_REWRITE_CONV[compile_repl_decs_eq] THENC eval)
+  ``repl_decs_code``)
+
+val call_dec = ``Tdec (Dlet (Plit Unit) (App Opapp (Var(Long"REPL""call_repl_step")) (Lit Unit)))``
+
+val compile_call_repl_step_def = zDefine`
+  compile_call_repl_step = compile_special (FST compile_repl_decs) ^call_dec`
+
+
+val _ = computeLib.add_thms [compilerProofTheory.compile_special_def,
+                             compilerProofTheory.prompt_to_i3_special_def] cs
+val eval_special = computeLib.CBV_CONV cs
+val compile_call_repl_step_eq = save_thm("compile_call_repl_step_eq",
+  time (REWR_CONV compile_call_repl_step_def THENC
+        PURE_ONCE_REWRITE_CONV[compile_repl_decs_eq] THENC
+        eval_special)
+  ``compile_call_repl_step``)
+
+val compile_call_repl_step_labels = store_thm("compile_call_repl_step_labels",
+  ``FILTER is_Label compile_call_repl_step = []``,
+  REWRITE_TAC[compile_call_repl_step_eq] THEN EVAL_TAC)
+
+val _ = Feedback.set_trace "TheoryPP.include_docs" 0
+val _ = export_theory()
